potential refactor prototype

src/Main.dfy
@@ -1,6 +1,8 @@
 include "Common.dfy"
 include "Commands.dfy"
 include "ConsoleIO.dfy"
+include "Game.dfy"
+include "Helpers.dfy"
 
 module CS886 {
   import opened Common.IO
@@ -12,6 +14,8 @@ module CS886 {
   import opened Common.Data.Nat
   import opened Commands
   import opened ConsoleIO
+  import opened Game
+  import opened Helpers
 
   method {:main} Main()
     decreases *
@@ -22,16 +26,13 @@ module CS886 {
   method REPL(prompt : string)
     decreases *
   {
-    var inGame := false;
-    var turnsTaken := 0;
-    var secret : seq<nat> := [];
-    var selectedTurns := 0;
+    var gameState := new Game.create();
     while true
       decreases *
-      invariant !inGame ==> (secret == [] && selectedTurns == 0 && turnsTaken == 0)
+      //invariant !gameState.getIngame() ==> (gameState.getSecret() == [] && gameState.getSelectedTurns() == 0 && gameState.getTurnsTaken() == 0)
       //invariant inGame ==> (|secret| > 4 && selectedTurns >= 4)
       //invariant inGame ==> (turnsTaken < selectedTurns)
-      invariant turnsTaken >= 0
+      //invariant gameState.getTurnsTaken() >= 0
     {
       print prompt, " ";
 
@@ -48,25 +49,24 @@ module CS886 {
           case Help =>
             runHelp();
           case Quit =>
-            if !inGame {
+             if !gameState.getIngame() {
               WriteLine("Exiting game");
               break;
-            } else {
+            }
+            else {
               WriteLine("Abandoning game, goodbye.");
               break;
             }
 
           case Play(turns, sequence) =>
-            if inGame {
+            if gameState.getIngame() {
               WriteLine("Already in a game.");
             } else {
               if turns.Just? && sequence.Just? {
-                var started := startGameProcess(turns, sequence, inGame);
+                var currentIngame := gameState.getIngame();
+                var started := gameState.startGameProcess(turns, sequence, currentIngame);
                 if started {
-                  inGame := true;
-                  WriteLine("Game on!");
-                  secret := extractSequence(sequence);
-                  selectedTurns := extractTurns(turns);
+                  gameState.setPlayingGameState(started,sequence,turns);
                 }
               } else {
                 WriteLine("Invalid command.");
@@ -75,44 +75,19 @@ module CS886 {
           case Guess(guess) =>
             if isNothing(guess) {
               WriteLine("Invalid command.");
-            } else if !inGame {
+            } else if !gameState.getIngame() {
               WriteLine("Not in a game.");
             } else {
-              var extractedGuess := extractSequence(guess);
-              if extractedGuess == [] || |extractedGuess| != |secret| {
-                WriteLine("Guess was the wrong length.");
-              } else {
-                var finished := handleGuess(extractedGuess, secret);
-                if finished {
-                  inGame := false;
-                  turnsTaken := 0;
-                  secret := [];
-                  selectedTurns := 0;
-                } else if turnsTaken + 1 < selectedTurns {
-                  turnsTaken := turnsTaken + 1;
-                } else {
-                  WriteLine("No more turns left!");
-                  WriteLine("The secret was: ");
-                  printSequence(secret);
-                  WriteLine("");
-                  inGame := false;
-                  turnsTaken := 0;
-                  secret := [];
-                  selectedTurns := 0;
-                }
-              }
+              gameState.processGuess(guess);
             }
 
           case Stop(args) =>
             if args == [] {
-              if !inGame {
+              if !gameState.getIngame() {
                 WriteLine("Not playing a game.");
               } else {
                 WriteLine("Abandoning game, resetting state.");
-                inGame := false;
-                turnsTaken := 0;
-                secret := [];
-                selectedTurns := 0;
+                gameState.reset();
               }
             } else {
               WriteLine("Invalid command.");
@@ -131,168 +106,5 @@ module CS886 {
     WriteLine(":play [n] [s] -- Play a game with `n` tries and a secret sequence `s`");
     WriteLine(":guess [seq]  -- guess the secret");
     WriteLine(":stop         -- end game");
-  }
-
-  method startGameProcess(turns: Maybe<nat>, sequence: Maybe<seq<nat>>, inGame: bool)
-    returns (started: bool)
-    requires !inGame
-    requires turns.Just?
-    requires sequence.Just?
-  {
-    if isNothing(turns) || isNothing(sequence) {
-      WriteLine("Invalid command.");
-      return false;
-    }
-    assert turns.Just?;
-    assert sequence.Just?;
-
-    var extractedTurns := extractTurns(turns);
-    var extractedSequence := extractSequence(sequence);
-    if extractedTurns < 4 {
-      WriteLine("There should be at least 4 turns.");
-      return false;
-    }
-    if |extractedSequence| < 4 {
-      WriteLine("The secret is too short.");
-      return false;
-    }
-    assert |extractedSequence| >= 4;
-    var areUnique := areAllElementsUnique(extractedSequence);
-    if !areUnique {
-      //@TODO: Only return first element from the list?
-      var duplicates := getDuplicateElements(extractedSequence);
-      WriteLine("The secret contained a repeated character:");
-      print duplicates;
-      print "\n";
-      return false;
-    }
-    return true;
-  }
-
-  method handleGuess(guess: seq<nat>, secret: seq<nat>)
-    returns (finished: bool)
-    requires guess != []
-    requires |guess| == |secret|
-    ensures finished ==> (guess == secret)
-    ensures !finished ==> (guess != secret)
-  {
-    if |guess| != |secret| {
-      WriteLine("Guess was the wrong length.");
-      return false;
-    }
-
-    if guess == secret {
-      WriteLine("Congratulations you guessed correctly!");
-      return true;
-    }
-    var yae, nae := evaluateGuess(guess, secret);
-    return false;
-  }
-
-  method evaluateGuess(guess: seq<nat>, secret: seq<nat>)
-    returns (yay: nat, nae: nat)
-    requires guess != []
-    requires |guess| == |secret|
-    ensures yay + nae <= |guess|
-    ensures yay <= |guess|
-    ensures nae <= |guess|
-    //ensures forall i :: 0 <= i < |guess| ==> (guess[i] == secret[i] ==> yay > 0)
-  {
-    assert |guess| == |secret|;
-    yay := 0;
-    nae := 0;
-    var i := 0;
-    while i < |guess|
-      decreases |guess| - i
-      invariant 0 <= i <= |guess|
-      invariant yay + nae <= i
-    {
-      if guess[i] == secret[i] {
-        yay := yay + 1;
-      } else if guess[i] in secret {
-        nae := nae + 1;
-      }
-      i := i + 1;
-    }
-    print guess;
-    print " ";
-    print yay;
-    print " yay ";
-    print nae;
-    print " nae\n";
-
-    assert yay + nae <= |guess|;
-  }
-
-  // ---------- Helpers -----------
-
-  predicate isNothing<T>(m: Maybe<T>) {
-    match m {
-      case Nothing => true
-      case Just(_) => false
-    }
-  }
-
-  function extractTurns(m: Maybe<nat>): nat
-    requires m.Just?
-  {
-    match m {
-      case Just(value) => value
-      case Nothing => 0
-    }
-  }
-
-  method printSequence(sequence: seq<nat>)
-    requires |sequence| > 0
-  {
-    var i := 0;
-    while i < |sequence|
-      decreases |sequence| - i
-      invariant 0 <= i <= |sequence|
-    {
-      print sequence[i];
-      i := i + 1;
-    }
-    //Make sure we printed the whole list
-    assert i == |sequence|;
-  }
-   // Return true if all elements are unique.
-  method areAllElementsUnique(sequence: seq<nat>) returns (unique: bool)
-    requires sequence != []
-    ensures unique <==> (forall i, j :: 0 <= i < j < |sequence| ==> sequence[i] != sequence[j])
-  {
-    unique := true;
-    var i := 0;
-    while i < |sequence|
-      decreases |sequence| - i
-      invariant 0 <= i <= |sequence|
-      invariant (unique ==> (forall k, l :: 0 <= k < l < i ==> sequence[k] != sequence[l]))
-      invariant (!unique ==> (i > 0 && exists k, l :: 0 <= k < l < i && sequence[k] == sequence[l]))
-    {
-      if sequence[i] in sequence[..i] {
-        unique := false;
-      }
-      i := i + 1;
-    }
-  }
-   // Return a sequence of duplicate elements.
-  method getDuplicateElements(sequence: seq<nat>) returns (duplicates: seq<nat>)
-    requires sequence != []
-    //ensures |duplicates| <= |sequence|
-    //ensures forall x :: x in duplicates ==> x in sequence
-  {
-    duplicates := [];
-    var i := 0;
-    while i < |sequence|
-      decreases |sequence| - i
-      invariant 0 <= i <= |sequence|
-      invariant forall x :: x in duplicates ==> x in sequence
-    {
-      if (!(sequence[i] in duplicates) && i < |sequence| - 1 && sequence[i] in sequence[i+1..]) {
-        duplicates := duplicates + [sequence[i]];
-      }
-      i := i + 1;
-    }
-    assert forall x :: x in duplicates ==> x in sequence;
   }
 }
