src/Game.dfy
@@ -1,0 +1,207 @@
+include "Helpers.dfy"
+include "Common.dfy"
+include "Commands.dfy"
+include "ConsoleIO.dfy"
+module Game {
+  import opened Helpers
+  import opened Common.IO
+  import opened Common.Data
+  import opened Common.Data.String
+  import opened Common.Data.Maybe
+  import opened Common.Data.Result
+  import opened Common.Data.Seq
+  import opened Common.Data.Nat
+  import opened Commands
+  import opened ConsoleIO
+  class Game {
+    var inGame:bool
+    var turnsTaken:nat
+    var secret : seq<nat>
+    var selectedTurns:nat
+
+    constructor create() {
+      inGame := false;
+      turnsTaken := 0;
+      secret := [];
+      selectedTurns := 0;
+    }
+    function getIngame():bool
+    reads this {
+        inGame
+    }
+    method setIngame(val:bool)
+    modifies this {
+        inGame := val;
+    }
+
+    function getTurnsTaken() : nat
+    reads this {
+      turnsTaken
+    }
+    method setTurnsTaken(val:nat)
+    modifies this {
+        turnsTaken := val;
+    }
+    method incrementTurnsTaken()
+    modifies this
+    {
+        turnsTaken := turnsTaken + 1;
+    }
+
+    function getSecret() : seq<nat>
+    reads this {
+      secret
+    }
+    method setSecret(val:seq<nat>)
+    modifies this
+    {
+        secret := val;
+    }
+    method reset()
+    ensures inGame == false
+    ensures turnsTaken == 0
+    ensures secret == []
+    ensures selectedTurns == 0
+    {
+      inGame := false;
+      turnsTaken := 0;
+      secret := [];
+      selectedTurns := 0;
+    }
+
+    function getSelectedTurns() : nat
+    reads this {
+      selectedTurns
+    }
+    method setSelectedTurns(val:nat)
+    modifies this
+    {
+      selectedTurns := val;
+    }
+
+    method startGameProcess(turns: Maybe<nat>, sequence: Maybe<seq<nat>>, inGame: bool)
+    returns (started: bool)
+    requires !inGame
+    requires turns.Just?
+    requires sequence.Just?
+    {
+      if isNothing(turns) || isNothing(sequence) {
+        WriteLine("Invalid command.");
+        return false;
+      }
+      assert turns.Just?;
+      assert sequence.Just?;
+
+      var extractedTurns := extractTurns(turns);
+      var extractedSequence := extractSequence(sequence);
+      if extractedTurns < 4 {
+        WriteLine("There should be at least 4 turns.");
+        return false;
+      }
+      if |extractedSequence| < 4 {
+        WriteLine("The secret is too short.");
+        return false;
+      }
+      assert |extractedSequence| >= 4;
+      var areUnique := areAllElementsUnique(extractedSequence);
+      if !areUnique {
+        //@TODO: Only return first element from the list?
+        var duplicates := getDuplicateElements(extractedSequence);
+        WriteLine("The secret contained a repeated character:");
+        print duplicates;
+        print "\n";
+        return false;
+      }
+      return true;
+    }
+    method setPlayingGameState(inGame:bool, secret:Maybe<seq<nat>>, selectedTurns:Maybe<nat>)
+    modifies this
+    requires secret.Just?
+    requires selectedTurns.Just?
+    requires inGame == true
+    {
+      this.setIngame(true);
+      WriteLine("Game on!");
+      var extractedSecret := extractSequence(secret);
+      var extractedTurns := extractTurns(selectedTurns);
+      this.setSecret(extractedSecret);
+      this.setSelectedTurns(extractedTurns);
+    }
+
+    method processGuess(guess: Maybe<seq<nat>>) {
+      var extractedGuess := extractSequence(guess);
+      if extractedGuess == [] || |extractedGuess| != |secret| {
+        WriteLine("Guess was the wrong length.");
+      } else {
+        var finished := handleGuess(extractedGuess, secret);
+        if finished {
+          this.reset();
+        } else if turnsTaken + 1 < selectedTurns {
+          this.incrementTurnsTaken();
+        } else {
+          this.forceEndGame();
+        }
+      }
+    }
+    method handleGuess(guess: seq<nat>, secret: seq<nat>)
+    returns (finished: bool)
+    requires guess != []
+    requires |guess| == |secret|
+    ensures finished ==> (guess == secret)
+    ensures !finished ==> (guess != secret)
+    {
+      if |guess| != |secret| {
+        WriteLine("Guess was the wrong length.");
+        return false;
+      }
+
+      if guess == secret {
+        WriteLine("Congratulations you guessed correctly!");
+        return true;
+      }
+      var yae, nae := evaluateGuess(guess, secret);
+      return false;
+    }
+    method evaluateGuess(guess: seq<nat>, secret: seq<nat>)
+    returns (yay: nat, nae: nat)
+    requires guess != []
+    requires |guess| == |secret|
+    ensures yay + nae <= |guess|
+    ensures yay <= |guess|
+    ensures nae <= |guess|
+    //ensures forall i :: 0 <= i < |guess| ==> (guess[i] == secret[i] ==> yay > 0)
+    {
+      assert |guess| == |secret|;
+      yay := 0;
+      nae := 0;
+      var i := 0;
+      while i < |guess|
+        decreases |guess| - i
+        invariant 0 <= i <= |guess|
+        invariant yay + nae <= i
+      {
+        if guess[i] == secret[i] {
+          yay := yay + 1;
+        } else if guess[i] in secret {
+          nae := nae + 1;
+        }
+        i := i + 1;
+      }
+      print guess;
+      print " ";
+      print yay;
+      print " yay ";
+      print nae;
+      print " nae\n";
+
+      assert yay + nae <= |guess|;
+    }
+    method forceEndGame() {
+      WriteLine("No more turns left!");
+      WriteLine("The secret was: ");
+      printSequence(secret);
+      WriteLine("");
+      this.reset();
+    }
+  }
+}
