src/Helpers.dfy
@@ -1,0 +1,79 @@
+include "Common.dfy"
+module Helpers {
+  import opened Common.IO
+  import opened Common.Data
+  import opened Common.Data.String
+  import opened Common.Data.Maybe
+  import opened Common.Data.Result
+  import opened Common.Data.Seq
+  import opened Common.Data.Nat
+  predicate isNothing<T>(m: Maybe<T>) {
+    match m {
+      case Nothing => true
+      case Just(_) => false
+    }
+  }
+
+  function extractTurns(m: Maybe<nat>): nat
+    requires m.Just?
+  {
+    match m {
+      case Just(value) => value
+      case Nothing => 0
+    }
+  }
+
+  method printSequence(sequence: seq<nat>)
+    requires |sequence| > 0
+  {
+    var i := 0;
+    while i < |sequence|
+      decreases |sequence| - i
+      invariant 0 <= i <= |sequence|
+    {
+      print sequence[i];
+      i := i + 1;
+    }
+    //Make sure we printed the whole list
+    assert i == |sequence|;
+  }
+   // Return true if all elements are unique.
+  method areAllElementsUnique(sequence: seq<nat>) returns (unique: bool)
+    requires sequence != []
+    ensures unique <==> (forall i, j :: 0 <= i < j < |sequence| ==> sequence[i] != sequence[j])
+  {
+    unique := true;
+    var i := 0;
+    while i < |sequence|
+      decreases |sequence| - i
+      invariant 0 <= i <= |sequence|
+      invariant (unique ==> (forall k, l :: 0 <= k < l < i ==> sequence[k] != sequence[l]))
+      invariant (!unique ==> (i > 0 && exists k, l :: 0 <= k < l < i && sequence[k] == sequence[l]))
+    {
+      if sequence[i] in sequence[..i] {
+        unique := false;
+      }
+      i := i + 1;
+    }
+  }
+   // Return a sequence of duplicate elements.
+  method getDuplicateElements(sequence: seq<nat>) returns (duplicates: seq<nat>)
+    requires sequence != []
+    //ensures |duplicates| <= |sequence|
+    //ensures forall x :: x in duplicates ==> x in sequence
+  {
+    duplicates := [];
+    var i := 0;
+    while i < |sequence|
+      decreases |sequence| - i
+      invariant 0 <= i <= |sequence|
+      invariant forall x :: x in duplicates ==> x in sequence
+    {
+      if (!(sequence[i] in duplicates) && i < |sequence| - 1 && sequence[i] in sequence[i+1..]) {
+        duplicates := duplicates + [sequence[i]];
+      }
+      i := i + 1;
+    }
+    assert forall x :: x in duplicates ==> x in sequence;
+  }
+}
